theories/LogicalRelation/Definition/Sig.v
@@ -19,6 +19,13 @@ Definition SigRedTyAdequate@{i j} `{ta : tag} `{WfContext ta} `{WfType ta} `{Con
 
 Module SigRedTyPack := ParamRedTyPack.
 
+Lemma fst_comp : forall {Γ A A' a Δ Ξ} {ρ : Δ ≤ Γ} {ρ' : Ξ ≤ Δ} {R}, [R | Ξ ||- a⟨ρ'∘w ρ⟩ ≅ a⟨ρ'∘w ρ⟩ : A ≅ A'] ->
+ [R | Ξ ||- a⟨ρ⟩⟨ρ'⟩ ≅ a⟨ρ⟩⟨ρ'⟩ : A].
+Proof.
+  intros * heq.
+  now rewrite wk_comp_ren_on.
+Defined.
+
 Inductive isLRPair `{ta : tag} `{WfContext ta}
   `{WfType ta} `{ConvType ta} `{RedType ta} `{Typing ta} `{ConvTerm ta} `{ConvNeuConv ta}
   {Γ : context} {A B : term} (ΣA : SigRedTyPack Γ A B) : term -> Type :=
@@ -30,11 +37,12 @@ Inductive isLRPair `{ta : tag} `{WfContext ta}
   (rfst : forall {Δ} (ρ : Δ ≤ Γ) (h : [ |- Δ ]),
       [ΣA.(PolyRedPack.shpRed) ρ h | Δ ||- a⟨ρ⟩ ≅ a⟨ρ⟩ : (SigRedTyPack.domL ΣA)⟨ρ⟩])
   (rsnd : forall {Δ} (ρ : Δ ≤ Γ) (h : [ |- Δ ]),
-      [Split_LRPack (ΣA.(PolyRedPack.posRed) ρ h (rfst ρ h))| Δ ||- b⟨ρ⟩ ≅ b⟨ρ⟩ : (SigRedTyPack.codL ΣA)[a⟨ρ⟩ .: (ρ >> tRel)] ]),
+      [Split_LRPack (ΣA.(PolyRedPack.posRed) ρ h (fun Ξ (ρ' : Ξ ≤ Δ) h'=> fst_comp (rfst (ρ'∘w ρ) h')))| Δ ||- b⟨ρ⟩ ≅ b⟨ρ⟩ : (SigRedTyPack.codL ΣA)[a⟨ρ⟩ .: (ρ >> tRel)] ]),
 
   isLRPair ΣA (tPair A' B' a b)
 
 | NeLRPair : forall p : term, [Γ |- p ~ p : SigRedTyPack.outTy ΣA] -> isLRPair ΣA p.
+
 
 Module SigRedTmEq.
 
@@ -64,6 +72,14 @@ Module SigRedTmEq.
     destruct ispair; constructor; now eapply convneu_whne.
   Defined.
 
+  Lemma fst_comp : forall {Γ A A' a a' Δ Ξ} {ρ : Δ ≤ Γ} {ρ' : Ξ ≤ Δ} {R}, [R | Ξ ||- tFst a⟨ρ'∘w ρ⟩ ≅ tFst a'⟨ρ'∘w ρ⟩ : A ≅ A'] ->
+   [R | Ξ ||- (tFst a⟨ρ⟩)⟨ρ'⟩ ≅ (tFst a'⟨ρ⟩)⟨ρ'⟩ : A].
+  Proof.
+    intros * heq.
+    do 2 rewrite <- wk_fst.
+    now do 2 rewrite wk_comp_ren_on.
+  Defined.
+
   Record SigRedTmEq `{ta : tag} `{WfContext ta}
     `{WfType ta} `{ConvType ta} `{RedType ta}
     `{Typing ta} `{ConvTerm ta} `{ConvNeuConv ta} `{RedTerm ta}
@@ -75,7 +91,7 @@ Module SigRedTmEq.
     eqFst [Δ] (ρ : Δ ≤ Γ) (h : [ |- Δ ]) :
       [ΣA.(PolyRedPack.shpRed) ρ h | Δ ||- tFst redL.(nf)⟨ρ⟩ ≅ tFst redR.(nf)⟨ρ⟩ : ΣA.(ParamRedTyPack.domL)⟨ρ⟩] ;
     eqSnd [Δ] (ρ : Δ ≤ Γ) (h : [ |- Δ ]) :
-      [Split_LRPack (ΣA.(PolyRedPack.posRed) ρ h (eqFst ρ h))| Δ ||- tSnd redL.(nf)⟨ρ⟩ ≅ tSnd redR.(nf)⟨ρ⟩ : _] ;
+      [Split_LRPack (ΣA.(PolyRedPack.posRed) ρ h (fun Ξ (ρ' : Ξ ≤ Δ) h'=> fst_comp (eqFst (ρ'∘w ρ) h')))| Δ ||- tSnd redL.(nf)⟨ρ⟩ ≅ tSnd redR.(nf)⟨ρ⟩ : _] ;
   }.
 
   Arguments SigRedTmEq {_ _ _ _ _ _ _ _ _ _ _ _}.
